finalize

term/term-project.v
@@ -11,7 +11,7 @@
    name: Bobbie Soedirgo
    student ID number: A0181001A
    e-mail address: sram-b@comp.nus.edu.sg
-*)
+ *)
 
 (* ********** *)
 
@@ -100,12 +100,12 @@ Beyond this absolute minimum, in decreasing importance, it would be good:
 Also, feel free to expand the source language and the target language,
 e.g., with multiplication, quotient, and modulo.
 
-*)
+ *)
 
 (* ********** *)
 
 Ltac fold_unfold_tactic name := intros; unfold name; fold name; reflexivity.
-  
+
 Require Import Arith Bool List String Ascii.
 
 (* caution: only use natural numbers up to 5000 *)
@@ -123,9 +123,9 @@ Definition string_of_nat (q0 : nat) : string :=
                            then s2
                            else let q3 := q2 / 10
                                 in let s2 := String (ascii_of_nat (48 + (q3 mod 10))) s2
-                        in if q3 <? 10
-                           then s2
-                           else "00000".
+                                   in if q3 <? 10
+                                      then s2
+                                      else "00000".
 
 Notation "A =n= B" := (beq_nat A B) (at level 70, right associativity).
 
@@ -155,7 +155,7 @@ Inductive expressible_value : Type :=
 
 Definition specification_of_evaluate (evaluate : arithmetic_expression -> expressible_value) :=
   (forall n : nat,
-     evaluate (Literal n) = Expressible_nat n)
+      evaluate (Literal n) = Expressible_nat n)
   /\
   ((forall (ae1 ae2 : arithmetic_expression)
            (s1 : string),
@@ -229,7 +229,7 @@ Admitted.
    a. time permitting, prove that each of the definitions above specifies at most one function;
    b. implement these two functions; and
    c. verify that each of your functions satisfies its specification.
-*)
+ *)
 
 Fixpoint evaluate_v0 (ae : arithmetic_expression) : expressible_value :=
   match ae with
@@ -317,40 +317,40 @@ Proof.
   - split.
     + split.
       * intros ae1 ae2 s1 H1_msg.
-        rewrite fold_unfold_evaluate_v0_Plus.
+        rewrite -> (fold_unfold_evaluate_v0_Plus ae1 ae2).
         rewrite H1_msg.
         reflexivity.
       * split.
         -- intros ae1 ae2 n1 s2 H1_nat H2_msg.
-           rewrite fold_unfold_evaluate_v0_Plus.
+           rewrite -> (fold_unfold_evaluate_v0_Plus ae1 ae2).
            rewrite H1_nat.
            rewrite H2_msg.
            reflexivity.
         -- intros ae1 ae2 n1 n2 H1_nat H2_nat.
-           rewrite fold_unfold_evaluate_v0_Plus.
+           rewrite -> (fold_unfold_evaluate_v0_Plus ae1 ae2).
            rewrite H1_nat.
            rewrite H2_nat.
            reflexivity.
     + split.
       * intros ae1 ae2 s1 H1_msg.
-        rewrite fold_unfold_evaluate_v0_Minus.
+        rewrite -> (fold_unfold_evaluate_v0_Minus ae1 ae2).
         rewrite H1_msg.
         reflexivity.
       * split.
         -- intros ae1 ae2 n1 s2 H1_nat H2_msg.
-           rewrite fold_unfold_evaluate_v0_Minus.
+           rewrite -> (fold_unfold_evaluate_v0_Minus ae1 ae2).
            rewrite H1_nat.
            rewrite H2_msg.
            reflexivity.
         -- split.
            ++ intros ae1 ae2 n1 n2 H1_nat H2_nat H_lt.
-              rewrite fold_unfold_evaluate_v0_Minus.
+              rewrite -> (fold_unfold_evaluate_v0_Minus ae1 ae2).
               rewrite H1_nat.
               rewrite H2_nat.
               rewrite H_lt.
               reflexivity.
            ++ intros ae1 ae2 n1 n2 H1_nat H2_nat H_gt.
-              rewrite fold_unfold_evaluate_v0_Minus.
+              rewrite -> (fold_unfold_evaluate_v0_Minus ae1 ae2).
               rewrite H1_nat.
               rewrite H2_nat.
               rewrite H_gt.
@@ -367,9 +367,8 @@ Theorem interpret_v0_satisfies_the_specification_of_interpret :
   specification_of_interpret interpret_v0.
 Proof.
   unfold specification_of_interpret, interpret_v0.
-  intros evaluate' S_evaluate' ae.
-  Check (there_is_at_most_one_evaluate_function evaluate_v0 evaluate' evaluate_v0_satisfies_the_specification_of_evaluate S_evaluate' ae).
-  exact (there_is_at_most_one_evaluate_function evaluate_v0 evaluate' evaluate_v0_satisfies_the_specification_of_evaluate S_evaluate' ae).
+  intros evaluate S_evaluate ae.
+  exact (there_is_at_most_one_evaluate_function evaluate_v0 evaluate evaluate_v0_satisfies_the_specification_of_evaluate S_evaluate ae).
 Qed.
 
 (* ********** *)
@@ -399,7 +398,7 @@ Inductive result_of_decoding_and_execution : Type :=
 Definition specification_of_decode_execute (decode_execute : byte_code_instruction -> data_stack -> result_of_decoding_and_execution) :=
   (forall (n : nat)
           (ds : data_stack),
-     decode_execute (PUSH n) ds = OK (n :: ds))
+      decode_execute (PUSH n) ds = OK (n :: ds))
   /\
   ((decode_execute ADD nil = KO "ADD: stack underflow")
    /\
@@ -430,7 +429,7 @@ Theorem there_is_at_most_one_decode_execute_function :
     specification_of_decode_execute decode_execute1 ->
     specification_of_decode_execute decode_execute2 ->
     forall (bci : byte_code_instruction)
-      (ds : data_stack),
+           (ds : data_stack),
       decode_execute1 bci ds = decode_execute2 bci ds.
 Proof.
 Admitted.
@@ -439,7 +438,7 @@ Admitted.
    a. time permitting, prove that the definition above specifies at most one function;
    b. implement this function; and
    c. verify that your function satisfies the specification.
-*)
+ *)
 
 Definition decode_execute_v0 (bcis : byte_code_instruction) (ds : data_stack) : result_of_decoding_and_execution :=
   match bcis with
@@ -452,7 +451,7 @@ Definition decode_execute_v0 (bcis : byte_code_instruction) (ds : data_stack) : 
     | n2 :: ds' =>
       match ds' with
       | nil =>
-      KO "ADD: stack underflow"
+        KO "ADD: stack underflow"
       | n1 :: ds'' =>
         OK ((n1 + n2) :: ds'')
       end
@@ -464,7 +463,7 @@ Definition decode_execute_v0 (bcis : byte_code_instruction) (ds : data_stack) : 
     | n2 :: ds' =>
       match ds' with
       | nil =>
-      KO "SUB: stack underflow"
+        KO "SUB: stack underflow"
       | n1 :: ds'' =>
         if n1 <? n2
         then KO (String.append "numerical underflow: -" (string_of_nat (n2 - n1)))
@@ -472,30 +471,28 @@ Definition decode_execute_v0 (bcis : byte_code_instruction) (ds : data_stack) : 
       end
     end
   end.
-    
+
 Theorem decode_execute_v0_satisfies_the_specification_of_decode_execute :
   specification_of_decode_execute decode_execute_v0.
 Proof.
   unfold specification_of_decode_execute, decode_execute_v0.
   split.
-  - reflexivity.
+  - intros n ds.
+    reflexivity.
   - split.
     + split.
       * reflexivity.
       * split.
-        -- reflexivity.
-        -- reflexivity.
+        -- intros _.
+           reflexivity.
+        -- intros n1 n2 ds.
+           reflexivity.
     + split.
       * reflexivity.
       * split.
-        -- reflexivity.
-        -- split.
-           ++ intros.
-              rewrite H.
-              reflexivity.
-           ++ intros.
-              rewrite H.
-              reflexivity.
+        -- intros _.
+           reflexivity.
+        -- split; intros n1 n2 ds H_lt; rewrite H_lt; reflexivity.
 Qed.
 
 (* ********** *)
@@ -528,7 +525,7 @@ Theorem there_is_at_most_one_fetch_decode_execute_loop_function :
     specification_of_fetch_decode_execute_loop fetch_decode_execute_loop1 ->
     specification_of_fetch_decode_execute_loop fetch_decode_execute_loop2 ->
     forall (bcis : list byte_code_instruction)
-      (ds : data_stack),
+           (ds : data_stack),
       fetch_decode_execute_loop1 bcis ds = fetch_decode_execute_loop2 bcis ds.
 Proof.
 Admitted.
@@ -537,7 +534,7 @@ Admitted.
    a. time permitting, prove that the definition above specifies at most one function;
    b. implement this function; and
    c. verify that your function satisfies the specification.
-*)
+ *)
 
 Fixpoint fetch_decode_execute_loop_v0 (bcis : list byte_code_instruction) (ds : data_stack) : result_of_decoding_and_execution :=
   match bcis with
@@ -562,8 +559,8 @@ Qed.
 
 Lemma fold_unfold_fetch_decode_execute_loop_v0_cons :
   forall (bci : byte_code_instruction)
-    (bcis' : list byte_code_instruction)
-    (ds : data_stack),
+         (bcis' : list byte_code_instruction)
+         (ds : data_stack),
     fetch_decode_execute_loop_v0 (bci :: bcis') ds =
     match decode_execute_v0 bci ds with
     | OK ds' =>
@@ -581,126 +578,34 @@ Proof.
   unfold specification_of_fetch_decode_execute_loop.
   intros decode_execute S_decode_execute.
   split.
-  (* bcis: nil case *)
+  (* bcis: nil *)
   - exact fold_unfold_fetch_decode_execute_loop_v0_nil.
-  (* bcis: cons case *)
+  (* bcis: cons *)
   - split. 
-    (* decode_execute: OK case *)
-    (* + intros [n | |] bcis'. *)
+    (* decode_execute: OK *)
     + intros bci bcis' ds ds' H_decode_execute.
-      rewrite fold_unfold_fetch_decode_execute_loop_v0_cons.
-      rewrite (there_is_at_most_one_decode_execute_function
-                 decode_execute
-                 decode_execute_v0
-                 S_decode_execute
-                 decode_execute_v0_satisfies_the_specification_of_decode_execute
-                 bci
-                 ds) in H_decode_execute.
+      rewrite -> (fold_unfold_fetch_decode_execute_loop_v0_cons bci bcis' ds).
+      rewrite -> (there_is_at_most_one_decode_execute_function
+                    decode_execute
+                    decode_execute_v0
+                    S_decode_execute
+                    decode_execute_v0_satisfies_the_specification_of_decode_execute
+                    bci
+                    ds) in H_decode_execute.
       rewrite H_decode_execute.
       reflexivity.
-    + 
-
-      
-      (* bci: PUSH case *)
-      * intros ds ds' H_decode_execute.
-        rewrite fold_unfold_fetch_decode_execute_loop_v0_cons.
-        unfold decode_execute_v0.
-        destruct S_decode_execute as [S_decode_execute _].
-        rewrite S_decode_execute in H_decode_execute.
-        injection H_decode_execute as H_ds.
-        rewrite H_ds.
-        reflexivity.
-      (* bci: ADD case *)
-      * intros [| n2 [| n1 ds']] ds'' H_decode_execute.
-        (* ds: nil case *)
-        -- destruct S_decode_execute as [_ [[S_decode_execute _] _]].
-           rewrite S_decode_execute in H_decode_execute.
-           discriminate H_decode_execute.
-        (* ds: n2 :: nil case *)
-        -- destruct S_decode_execute as [_ [[_ [S_decode_execute _]] _]].
-           rewrite S_decode_execute in H_decode_execute.
-           discriminate H_decode_execute.
-        (* ds: n2 :: n1 :: nil case *)
-        -- destruct S_decode_execute as [_ [[_ [_ S_decode_execute]] _]].
-           rewrite S_decode_execute in H_decode_execute.
-           rewrite fold_unfold_fetch_decode_execute_loop_v0_cons.
-           unfold decode_execute_v0.
-           injection H_decode_execute as H.
-           rewrite H.
-           reflexivity.
-      (* bci: SUB case *)
-      * intros [| n2 [| n1 ds']] ds'' H_decode_execute.
-        (* ds: nil case *)
-        -- destruct S_decode_execute as [_ [_ [H _]]].
-           rewrite H in H_decode_execute.
-           discriminate H_decode_execute.
-        (* ds: n2 :: nil case *)
-        -- destruct S_decode_execute as [_ [_ [_ [H _]]]].
-           rewrite H in H_decode_execute.
-           discriminate H_decode_execute.
-        (* ds: n2 :: n1 :: nil case *)
-        -- case (n1 <? n2) eqn:H_n.
-           ++ destruct S_decode_execute as [_ [_ [_ [_ [H _]]]]].
-              rewrite (H n1 n2 ds' H_n) in H_decode_execute.
-              discriminate H_decode_execute.
-           ++ destruct S_decode_execute as [_ [_ [_ [_ [_ H]]]]].
-              rewrite (H n1 n2 ds' H_n) in H_decode_execute.
-              injection H_decode_execute as H_n_sub.
-              rewrite fold_unfold_fetch_decode_execute_loop_v0_cons.
-              unfold decode_execute_v0.
-              rewrite H_n.
-              rewrite H_n_sub.
-              reflexivity.
-    (* decode_execute: KO case *)
-    + intros [n | |] bcis'.
-      (* bci: PUSH case *)
-      * intros ds s H_decode_execute.
-        destruct S_decode_execute as [S_decode_execute _].
-        rewrite S_decode_execute in H_decode_execute.
-        discriminate H_decode_execute.
-      (* bci: ADD case *)
-      * intros [| n2 [| n1 ds']] ds'' H_decode_execute.
-        (* ds: nil case *)
-        -- destruct S_decode_execute as [_ [[S_decode_execute _] _]].
-           rewrite S_decode_execute in H_decode_execute.
-           rewrite fold_unfold_fetch_decode_execute_loop_v0_cons.
-           unfold decode_execute_v0.
-           exact H_decode_execute.
-        (* ds: n2 :: nil case *)
-        -- destruct S_decode_execute as [_ [[_ [S_decode_execute _]] _]].
-           rewrite S_decode_execute in H_decode_execute.
-           rewrite fold_unfold_fetch_decode_execute_loop_v0_cons.
-           unfold decode_execute_v0.
-           exact H_decode_execute.
-        (* ds: n2 :: n1 :: nil case *)
-        -- destruct S_decode_execute as [_ [[_ [_ S_decode_execute]] _]].
-           rewrite S_decode_execute in H_decode_execute.
-           discriminate H_decode_execute.
-      (* bci: SUB case *)
-      * intros [| n2 [| n1 ds']] ds'' H_decode_execute.
-        (* ds: nil case *)
-        -- destruct S_decode_execute as [_ [_ [S_decode_execute _]]].
-           rewrite S_decode_execute in H_decode_execute.
-           rewrite fold_unfold_fetch_decode_execute_loop_v0_cons.
-           unfold decode_execute_v0.
-           exact H_decode_execute.
-        (* ds: n2 :: nil case *)
-        -- destruct S_decode_execute as [_ [_ [_ [S_decode_execute _]]]].
-           rewrite S_decode_execute in H_decode_execute.
-           rewrite fold_unfold_fetch_decode_execute_loop_v0_cons.
-           unfold decode_execute_v0.
-           exact H_decode_execute.
-        (* ds: n2 :: n1 :: nil case *)
-        -- case (n1 <? n2) eqn:H_n.
-           ++ destruct S_decode_execute as [_ [_ [_ [_ [H _]]]]].
-              rewrite (H n1 n2 ds' H_n) in H_decode_execute.
-              rewrite fold_unfold_fetch_decode_execute_loop_v0_cons.
-              unfold decode_execute_v0.
-              rewrite H_n.
-              exact H_decode_execute.
-           ++ destruct S_decode_execute as [_ [_ [_ [_ [_ H]]]]].
-              rewrite (H n1 n2 ds' H_n) in H_decode_execute.
-              discriminate H_decode_execute.
+    (* decode_execute: KO *)
+    + intros bci bcis' ds s H_decode_execute.
+      rewrite -> (fold_unfold_fetch_decode_execute_loop_v0_cons bci bcis' ds).
+      rewrite -> (there_is_at_most_one_decode_execute_function
+                    decode_execute
+                    decode_execute_v0
+                    S_decode_execute
+                    decode_execute_v0_satisfies_the_specification_of_decode_execute
+                    bci
+                    ds) in H_decode_execute.
+      rewrite H_decode_execute.
+      reflexivity.
 Qed.
 
 (* ********** *)
@@ -712,7 +617,7 @@ Qed.
    gives the same result as
    (1) executing bcis1 with ds, and then
    (2) executing bcis2 with the resulting data stack, if there exists one.
-*)
+ *)
 
 Lemma fold_unfold_append_nil :
   forall bcis2 : list byte_code_instruction,
@@ -734,89 +639,81 @@ Proposition fetch_decode_execute_loop_v0_and_append_commute :
   forall (bcis1 bcis2 : list byte_code_instruction)
          (ds1 : data_stack),
     (forall (ds2 : data_stack),
-       fetch_decode_execute_loop_v0 bcis1 ds1 = OK ds2 ->
-       fetch_decode_execute_loop_v0 (bcis1 ++ bcis2) ds1 = fetch_decode_execute_loop_v0 bcis2 ds2)
+        fetch_decode_execute_loop_v0 bcis1 ds1 = OK ds2 ->
+        fetch_decode_execute_loop_v0 (bcis1 ++ bcis2) ds1 = fetch_decode_execute_loop_v0 bcis2 ds2)
     /\
     (forall (s : string),
-       fetch_decode_execute_loop_v0 bcis1 ds1 = KO s ->
-       fetch_decode_execute_loop_v0 (bcis1 ++ bcis2) ds1 = KO s).
+        fetch_decode_execute_loop_v0 bcis1 ds1 = KO s ->
+        fetch_decode_execute_loop_v0 (bcis1 ++ bcis2) ds1 = KO s).
 Proof.
   intro bcis1.
-  induction bcis1 as [| bci1 bcis1' IH1].
+  induction bcis1 as [| bci1 bcis1' IHbcis1'].
   (* bcis1: nil *)
   - intros bcis2 ds1.
     split.
     (* OK *)
     + intros ds2 H_fdel.
-      rewrite fold_unfold_append_nil.
-      rewrite fold_unfold_fetch_decode_execute_loop_v0_nil in H_fdel.
+      rewrite -> (fold_unfold_append_nil bcis2).
+      rewrite -> (fold_unfold_fetch_decode_execute_loop_v0_nil ds1) in H_fdel.
       injection H_fdel as H_ds.
       rewrite H_ds.
       reflexivity.
     (* KO *)
     + intros s H_fdel.
-      rewrite fold_unfold_fetch_decode_execute_loop_v0_nil in H_fdel.
+      rewrite -> (fold_unfold_fetch_decode_execute_loop_v0_nil ds1) in H_fdel.
       discriminate H_fdel.
   (* bcis1: cons *)
   - split.
     (* OK *)
     + intros ds2 H_fdel.
-      rewrite fold_unfold_fetch_decode_execute_loop_v0_cons in H_fdel.
-      rewrite fold_unfold_append_cons.
-      rewrite fold_unfold_fetch_decode_execute_loop_v0_cons.
+      rewrite -> (fold_unfold_fetch_decode_execute_loop_v0_cons bci1 bcis1' ds1) in H_fdel.
+      unfold decode_execute_v0 in H_fdel.
+      rewrite -> (fold_unfold_append_cons bci1 bcis1' bcis2).
+      rewrite -> (fold_unfold_fetch_decode_execute_loop_v0_cons bci1 (bcis1' ++ bcis2)).
+      unfold decode_execute_v0.
       case bci1 as [n | |].
       (* bci: PUSH *)
-      * unfold decode_execute_v0 in H_fdel.
-        unfold decode_execute_v0.
-        destruct (IH1 bcis2 (n :: ds1)) as [H _].
-        exact (H ds2 H_fdel).
+      * destruct (IHbcis1' bcis2 (n :: ds1)) as [IHbcis1'_OK _].
+        exact (IHbcis1'_OK ds2 H_fdel).
       (* bci: ADD *)
-      * unfold decode_execute_v0 in H_fdel.
-        unfold decode_execute_v0.
-        case ds1 as [| n2 [| n1 ds']].
+      * case ds1 as [| n2 [| n1 ds1']].
         -- discriminate H_fdel.
         -- discriminate H_fdel.
-        -- destruct (IH1 bcis2 (n1 + n2 :: ds')) as [H _].
-           exact (H ds2 H_fdel).
+        -- destruct (IHbcis1' bcis2 (n1 + n2 :: ds1')) as [IHbcis1'_OK _].
+           exact (IHbcis1'_OK ds2 H_fdel).
       (* bci: SUB *)
-      * unfold decode_execute_v0 in H_fdel.
-        unfold decode_execute_v0.
-        case ds1 as [| n2 [| n1 ds1']].
+      * case ds1 as [| n2 [| n1 ds1']].
         -- discriminate H_fdel.
         -- discriminate H_fdel.
-        -- case (n1 <? n2) eqn:H_n.
+        -- case (n1 <? n2) eqn:H_lt.
            ++ discriminate H_fdel.
-           ++ destruct (IH1 bcis2 (n1 - n2 :: ds1')) as [H _].
-              exact (H ds2 H_fdel).
+           ++ destruct (IHbcis1' bcis2 (n1 - n2 :: ds1')) as [IHbcis1'_OK _].
+              exact (IHbcis1'_OK ds2 H_fdel).
     (* KO *)
     + intros s H_fdel.
-      rewrite fold_unfold_fetch_decode_execute_loop_v0_cons in H_fdel.
-      rewrite fold_unfold_append_cons.
-      rewrite fold_unfold_fetch_decode_execute_loop_v0_cons.
+      rewrite -> (fold_unfold_fetch_decode_execute_loop_v0_cons bci1 bcis1' ds1) in H_fdel.
+      unfold decode_execute_v0 in H_fdel.
+      rewrite -> (fold_unfold_append_cons bci1 bcis1' bcis2).
+      rewrite -> (fold_unfold_fetch_decode_execute_loop_v0_cons bci1 (bcis1' ++ bcis2) ds1).
+      unfold decode_execute_v0.
       case bci1 as [n | |].
       (* bci1: PUSH *)
-      * unfold decode_execute_v0 in H_fdel.
-        unfold decode_execute_v0.
-        destruct (IH1 bcis2 (n :: ds1)) as [_ H].
-        exact (H s H_fdel).
+      * destruct (IHbcis1' bcis2 (n :: ds1)) as [_ IHbcis1'_KO].
+        exact (IHbcis1'_KO s H_fdel).
       (* bci: ADD *)
-      * unfold decode_execute_v0 in H_fdel.
-        unfold decode_execute_v0.
-        case ds1 as [| n2 [| n1 ds1']].
+      * case ds1 as [| n2 [| n1 ds1']].
         -- exact H_fdel.
         -- exact H_fdel.
-        -- destruct (IH1 bcis2 (n1 + n2 :: ds1')) as [_ H].
-           exact (H s H_fdel).
+        -- destruct (IHbcis1' bcis2 (n1 + n2 :: ds1')) as [_ IHbcis1'_KO].
+           exact (IHbcis1'_KO s H_fdel).
       (* bci: SUB *)
-      * unfold decode_execute_v0 in H_fdel.
-        unfold decode_execute_v0.
-        case ds1 as [| n2 [| n1 ds1']].
+      * case ds1 as [| n2 [| n1 ds1']].
         -- exact H_fdel.
         -- exact H_fdel.
-        -- case (n1 <? n2) eqn:H_n.
+        -- case (n1 <? n2) eqn:H_lt.
            ++ exact H_fdel.
-           ++ destruct (IH1 bcis2 (n1 - n2 :: ds1')) as [_ H].
-              exact (H s H_fdel).
+           ++ destruct (IHbcis1' bcis2 (n1 - n2 :: ds1')) as [_ IHbcis1'_KO].
+              exact (IHbcis1'_KO s H_fdel).
 Qed.
 
 (* ********** *)
@@ -825,24 +722,24 @@ Definition specification_of_run (run : target_program -> expressible_value) :=
   forall fetch_decode_execute_loop : list byte_code_instruction -> data_stack -> result_of_decoding_and_execution,
     specification_of_fetch_decode_execute_loop fetch_decode_execute_loop ->
     (forall (bcis : list byte_code_instruction),
-       fetch_decode_execute_loop bcis nil = OK nil ->
-       run (Target_program bcis) = Expressible_msg "no result on the data stack")
+        fetch_decode_execute_loop bcis nil = OK nil ->
+        run (Target_program bcis) = Expressible_msg "no result on the data stack")
     /\
     (forall (bcis : list byte_code_instruction)
             (n : nat),
-       fetch_decode_execute_loop bcis nil = OK (n :: nil) ->
-       run (Target_program bcis) = Expressible_nat n)
+        fetch_decode_execute_loop bcis nil = OK (n :: nil) ->
+        run (Target_program bcis) = Expressible_nat n)
     /\
     (forall (bcis : list byte_code_instruction)
             (n n' : nat)
             (ds'' : data_stack),
-       fetch_decode_execute_loop bcis nil = OK (n :: n' :: ds'') ->
-       run (Target_program bcis) = Expressible_msg "too many results on the data stack")
+        fetch_decode_execute_loop bcis nil = OK (n :: n' :: ds'') ->
+        run (Target_program bcis) = Expressible_msg "too many results on the data stack")
     /\
     (forall (bcis : list byte_code_instruction)
             (s : string),
-       fetch_decode_execute_loop bcis nil = KO s ->
-       run (Target_program bcis) = Expressible_msg s).
+        fetch_decode_execute_loop bcis nil = KO s ->
+        run (Target_program bcis) = Expressible_msg s).
 
 Theorem there_is_at_most_one_run_function :
   forall (run1 run2 : target_program -> expressible_value),
@@ -857,7 +754,7 @@ Admitted.
    a. time permitting, prove that the definition above specifies at most one function;
    b. implement this function; and
    c. verify that your function satisfies the specification.
-*)
+ *)
 
 Definition run_v0 (tp : target_program) : expressible_value :=
   match tp with
@@ -880,7 +777,6 @@ Definition run_v0 (tp : target_program) : expressible_value :=
     end
   end.
 
-
 Theorem run_v0_satisfies_the_specification_of_run :
   specification_of_run run_v0.
 Proof.
@@ -888,48 +784,64 @@ Proof.
   intros fdel S_fdel.
   split.
   (* fdel: OK nil *)
-  - intro bcis.
-    induction bcis as [| bci bcis' IH].
-    + intro H_fdel.
-      rewrite fold_unfold_fetch_decode_execute_loop_v0_nil.
-      reflexivity.
-    + intro H_fdel.
-      rewrite fold_unfold_fetch_decode_execute_loop_v0_cons.
-      unfold decode_execute_v0.
-      case bci as [n | |].
-      (* bci: PUSH *)
-      * destruct (S_fdel
-                    decode_execute_v0
-                    decode_execute_v0_satisfies_the_specification_of_decode_execute) as [_ [H _]].
-        unfold decode_execute_v0 in H.
-        rewrite (H (PUSH n) bcis' nil nil) in H_fdel.
-        admit.
-        admit.
-      (* bci: ADD *)
-      * admit.
-      (* bci: SUB *)
-      * admit.
+  - intros bcis H_fdel.
+    rewrite -> (there_is_at_most_one_fetch_decode_execute_loop_function
+                  fdel
+                  fetch_decode_execute_loop_v0
+                  S_fdel
+                  fetch_decode_execute_loop_v0_satisfies_the_specification_of_fetch_decode_execute_loop
+                  bcis
+                  nil) in H_fdel.
+    rewrite H_fdel.
+    reflexivity.
   - split.
-    (* fdel: OK (n2 :: nil) *)
-     + admit.
-     + split.
-       (* fdel: OK (n2 :: n1 :: nil) *)
-       * admit.
-       (* fdel: KO *)
-       * admit.
-Admitted.
+    (* fdel: OK (n :: nil) *)
+    + intros bcis n H_fdel.
+      rewrite -> (there_is_at_most_one_fetch_decode_execute_loop_function
+                    fdel
+                    fetch_decode_execute_loop_v0
+                    S_fdel
+                    fetch_decode_execute_loop_v0_satisfies_the_specification_of_fetch_decode_execute_loop
+                    bcis
+                    nil) in H_fdel.
+      rewrite H_fdel.
+      reflexivity.
+    + split.
+      (* fdel: OK (n :: n' :: nil) *)
+      * intros bcis n n' ds'' H_fdel.
+        rewrite -> (there_is_at_most_one_fetch_decode_execute_loop_function
+                      fdel
+                      fetch_decode_execute_loop_v0
+                      S_fdel
+                      fetch_decode_execute_loop_v0_satisfies_the_specification_of_fetch_decode_execute_loop
+                      bcis
+                      nil) in H_fdel.
+        rewrite H_fdel.
+        reflexivity.
+      (* fdel: KO s *)
+      * intros bcis s H_fdel.
+        rewrite -> (there_is_at_most_one_fetch_decode_execute_loop_function
+                      fdel
+                      fetch_decode_execute_loop_v0
+                      S_fdel
+                      fetch_decode_execute_loop_v0_satisfies_the_specification_of_fetch_decode_execute_loop
+                      bcis
+                      nil) in H_fdel.
+        rewrite H_fdel.
+        reflexivity.
+Qed.
 
 (* ********** *)
 
 Definition specification_of_compile_aux (compile_aux : arithmetic_expression -> list byte_code_instruction) :=
   (forall n : nat,
-     compile_aux (Literal n) = PUSH n :: nil)
+      compile_aux (Literal n) = PUSH n :: nil)
   /\
   (forall ae1 ae2 : arithmetic_expression,
-     compile_aux (Plus ae1 ae2) = (compile_aux ae1) ++ (compile_aux ae2) ++ (ADD :: nil))
+      compile_aux (Plus ae1 ae2) = (compile_aux ae1) ++ (compile_aux ae2) ++ (ADD :: nil))
   /\
   (forall ae1 ae2 : arithmetic_expression,
-     compile_aux (Minus ae1 ae2) = (compile_aux ae1) ++ (compile_aux ae2) ++ (SUB :: nil)).
+      compile_aux (Minus ae1 ae2) = (compile_aux ae1) ++ (compile_aux ae2) ++ (SUB :: nil)).
 
 Theorem there_is_at_most_one_compile_aux_function :
   forall (compile_aux1 compile_aux2 : arithmetic_expression -> list byte_code_instruction),
@@ -944,7 +856,7 @@ Admitted.
    a. time permitting, prove that the definition above specifies at most one function;
    b. implement this function using list concatenation, i.e., ++; and
    c. verify that your function satisfies the specification.
-*)
+ *)
 
 Fixpoint compile_v0_aux (ae : arithmetic_expression) : list byte_code_instruction :=
   match ae with
@@ -985,7 +897,16 @@ Qed.
 Theorem compile_v0_aux_satisfies_the_specification_of_compile_aux :
   specification_of_compile_aux compile_v0_aux.
 Proof.
-Admitted.
+  unfold specification_of_compile_aux.
+  split.
+  (* Literal *)
+  - exact fold_unfold_compile_v0_aux_Literal.
+  - split.
+    (* Plus *)
+    + exact fold_unfold_compile_v0_aux_Plus.
+    (* Minus *)
+    + exact fold_unfold_compile_v0_aux_Minus.
+Qed.
 
 Definition specification_of_compile (compile : source_program -> target_program) :=
   forall compile_aux : arithmetic_expression -> list byte_code_instruction,
@@ -1006,7 +927,7 @@ Admitted.
    a. time permitting, prove that the definition above specifies at most one function;
    b. implement this function; and
    c. verify that your function satisfies the specification.
-*)
+ *)
 
 Definition compile_v0 (sp : source_program) : target_program :=
   match sp with
@@ -1017,7 +938,16 @@ Definition compile_v0 (sp : source_program) : target_program :=
 Theorem compile_v0_satisfies_the_specification_of_compile :
   specification_of_compile compile_v0.
 Proof.
-Admitted.
+  unfold specification_of_compile, compile_v0.
+  intros compile_aux S_compile_aux ae.
+  rewrite -> (there_is_at_most_one_compile_aux_function
+                compile_aux
+                compile_v0_aux
+                S_compile_aux
+                compile_v0_aux_satisfies_the_specification_of_compile_aux
+                ae).
+  reflexivity.
+Qed.
 
 (* Task 8:
    implement an alternative compiler
@@ -1028,162 +958,265 @@ Admitted.
    Subsidiary question:
    Are your compiler and your alternative compiler equivalent?
    How can you tell?
-*)
+ *)
 
-Fixpoint compile_v1_aux_aux (ae : arithmetic_expression) (bcis : list byte_code_instruction) : list byte_code_instruction :=
+Fixpoint compile_v1_aux (ae : arithmetic_expression) (bcis : list byte_code_instruction) : list byte_code_instruction :=
   match ae with
   | Literal n =>
     PUSH n :: bcis
   | Plus ae1 ae2 =>
-    compile_v1_aux_aux ae1 (compile_v1_aux_aux ae2 (ADD :: bcis))
+    compile_v1_aux ae1 (compile_v1_aux ae2 (ADD :: bcis))
   | Minus ae1 ae2 =>
-    compile_v1_aux_aux ae1 (compile_v1_aux_aux ae2 (SUB :: bcis))
+    compile_v1_aux ae1 (compile_v1_aux ae2 (SUB :: bcis))
   end.
 
-Compute compile_v1_aux_aux (Plus (Literal 1) (Minus (Literal 2) (Literal 3))) nil.
+Compute compile_v1_aux (Plus (Literal 1) (Minus (Literal 2) (Literal 3))) nil.
 
-Lemma fold_unfold_compile_v1_aux_aux_Literal :
+Lemma fold_unfold_compile_v1_aux_Literal :
   forall (n : nat)
-    (bcis : list byte_code_instruction),
-    compile_v1_aux_aux (Literal n) bcis =
+         (bcis : list byte_code_instruction),
+    compile_v1_aux (Literal n) bcis =
     PUSH n :: bcis.
 Proof.
-  fold_unfold_tactic compile_v1_aux_aux.
+  fold_unfold_tactic compile_v1_aux.
 Qed.
 
-Lemma fold_unfold_compile_v1_aux_aux_Plus :
+Lemma fold_unfold_compile_v1_aux_Plus :
   forall (ae1 ae2 : arithmetic_expression)
-    (bcis : list byte_code_instruction),
-    compile_v1_aux_aux (Plus ae1 ae2) bcis =
-    compile_v1_aux_aux ae1 (compile_v1_aux_aux ae2 (ADD :: bcis)).
+         (bcis : list byte_code_instruction),
+    compile_v1_aux (Plus ae1 ae2) bcis =
+    compile_v1_aux ae1 (compile_v1_aux ae2 (ADD :: bcis)).
 Proof.
-  fold_unfold_tactic compile_v1_aux_aux.
+  fold_unfold_tactic compile_v1_aux.
 Qed.
 
-Lemma fold_unfold_compile_v1_aux_aux_Minus :
+Lemma fold_unfold_compile_v1_aux_Minus :
   forall (ae1 ae2 : arithmetic_expression)
-    (bcis : list byte_code_instruction),
-    compile_v1_aux_aux (Minus ae1 ae2) bcis =
-    compile_v1_aux_aux ae1 (compile_v1_aux_aux ae2 (SUB :: bcis)).
+         (bcis : list byte_code_instruction),
+    compile_v1_aux (Minus ae1 ae2) bcis =
+    compile_v1_aux ae1 (compile_v1_aux ae2 (SUB :: bcis)).
 Proof.
-  fold_unfold_tactic compile_v1_aux_aux.
+  fold_unfold_tactic compile_v1_aux.
 Qed.
-
-Definition compile_v1_aux (ae : arithmetic_expression) : list byte_code_instruction :=
-  compile_v1_aux_aux ae nil.
-
-Theorem compile_v1_aux_satisfies_the_specification_of_compile_aux :
-  specification_of_compile_aux compile_v1_aux.
-Proof.
-  unfold specification_of_compile_aux, compile_v1_aux.
-  split.
-  - intro n.
-    rewrite fold_unfold_compile_v1_aux_aux_Literal.
-    reflexivity.
-  - split.
-    (* Plus case *)
-    + admit.
-    (* Minus case *)
-    + admit.
-Admitted.
 
 Definition compile_v1 (sp : source_program) : target_program :=
   match sp with
   | Source_program ae =>
-    Target_program (compile_v1_aux ae)
+    Target_program (compile_v1_aux ae nil)
   end.
+
+Lemma about_compile_v0_aux_and_compile_v1_aux :
+  forall (ae : arithmetic_expression)
+         (acc : list byte_code_instruction),
+    compile_v0_aux ae ++ acc = compile_v1_aux ae acc. 
+Proof.
+  intro ae.
+  induction ae as [n | ae1 IH1 ae2 IH2 | ae1 IH1 ae2 IH2].
+  - intro acc.
+    rewrite -> (fold_unfold_compile_v0_aux_Literal n).
+    rewrite -> (fold_unfold_append_cons (PUSH n) nil acc).
+    rewrite -> (app_nil_l acc).
+    rewrite -> (fold_unfold_compile_v1_aux_Literal n acc).
+    reflexivity.
+  - intro acc.
+    rewrite -> (fold_unfold_compile_v0_aux_Plus ae1 ae2).
+    rewrite -> (fold_unfold_compile_v1_aux_Plus ae1 ae2 acc).
+    Search ((_ ++ _) ++ _).
+    rewrite -> (app_assoc_reverse (compile_v0_aux ae1) (compile_v0_aux ae2 ++ ADD :: nil)).
+    rewrite -> (app_assoc_reverse (compile_v0_aux ae2) (ADD :: nil)).
+    rewrite -> (fold_unfold_append_cons ADD nil acc).
+    rewrite -> (app_nil_l acc).
+    rewrite -> (IH1 (compile_v0_aux ae2 ++ ADD :: acc)).
+    rewrite -> (IH2 (ADD :: acc)).
+    reflexivity.
+  - intro acc.
+    rewrite -> (fold_unfold_compile_v0_aux_Minus ae1 ae2).
+    rewrite -> (fold_unfold_compile_v1_aux_Minus ae1 ae2 acc).
+    Search ((_ ++ _) ++ _).
+    rewrite -> (app_assoc_reverse (compile_v0_aux ae1) (compile_v0_aux ae2 ++ SUB :: nil)).
+    rewrite -> (app_assoc_reverse (compile_v0_aux ae2) (SUB :: nil)).
+    rewrite -> (fold_unfold_append_cons SUB nil acc).
+    rewrite -> (app_nil_l acc).
+    rewrite -> (IH1 (compile_v0_aux ae2 ++ SUB :: acc)).
+    rewrite -> (IH2 (SUB :: acc)).
+    reflexivity.
+Qed.
+
+Theorem compile_v1_satisfies_the_specification_of_compile :
+  specification_of_compile compile_v1.
+Proof.
+  unfold specification_of_compile, compile_v1.
+  intros compile_aux S_compile_aux ae.
+  rewrite <- (about_compile_v0_aux_and_compile_v1_aux
+                ae nil).
+  rewrite -> (app_nil_r (compile_v0_aux ae)).
+  rewrite -> (there_is_at_most_one_compile_aux_function
+                compile_aux
+                compile_v0_aux
+                S_compile_aux
+                compile_v0_aux_satisfies_the_specification_of_compile_aux
+                ae).
+  reflexivity.
+Qed.
 
 (* ********** *)
 
 (* Task 9 (the capstone):
    Prove that interpreting an arithmetic expression gives the same result
    as first compiling it and then executing the compiled program.
-*)
+ *)
 
 Lemma about_the_commutative_diagram :
   forall ae : arithmetic_expression,
-    (exists n : nat,
-        evaluate_v0 ae = Expressible_nat n
-        /\
-        fetch_decode_execute_loop_v0 (compile_v0_aux ae) nil = OK (n :: nil))
-    \/
-    (exists s : string,
-        evaluate_v0 ae = Expressible_msg s
-        /\
-        fetch_decode_execute_loop_v0 (compile_v0_aux ae) nil = KO s).
+    (forall n : nat,
+        evaluate_v0 ae = Expressible_nat n ->
+        forall ds : data_stack,
+          fetch_decode_execute_loop_v0 (compile_v0_aux ae) ds = OK (n :: ds))
+    /\
+    (forall s : string,
+        evaluate_v0 ae = Expressible_msg s ->
+        forall ds : data_stack,
+          fetch_decode_execute_loop_v0 (compile_v0_aux ae) ds = KO s).
 Proof.
   intro ae.
   induction ae as [n |
-                   ae1 [[n1 [IH1_i IH1_c]] | [s1 [IH1_i IH1_c]]] ae2 [[n2 [IH2_i IH2_c]] | [s2 [IH2_i IH2_c]]] |
-                   ae1 [[n1 [IH1_i IH1_c]] | [s1 [IH1_i IH1_c]]] ae2 [[n2 [IH2_i IH2_c]] | [s2 [IH2_i IH2_c]]]].
-  (* Literal *)
-  - left.
-    exists n.
-    split.
-    + rewrite fold_unfold_evaluate_v0_Literal.
-      reflexivity.
-    + rewrite fold_unfold_compile_v0_aux_Literal.
-      rewrite fold_unfold_fetch_decode_execute_loop_v0_cons.
+                   ae1 [IH1_OK IH1_KO] ae2 [IH2_OK IH2_KO] |
+                   ae1 [IH1_OK IH1_KO] ae2 [IH2_OK IH2_KO]].
+  - split.
+    + intros n' H_evaluate ds.
+      rewrite -> (fold_unfold_evaluate_v0_Literal n) in H_evaluate.
+      injection H_evaluate as H_n.
+      rewrite -> (fold_unfold_compile_v0_aux_Literal n).
+      rewrite -> (fold_unfold_fetch_decode_execute_loop_v0_cons (PUSH n) nil ds).
       unfold decode_execute_v0.
-      exact (fold_unfold_fetch_decode_execute_loop_v0_nil (n :: nil)).
-  (* Plus nat nat *)
-  - admit.
-  (* Plus nat msg *)
-  - right.
-    exists s2.
-    rewrite fold_unfold_evaluate_v0_Plus.
-    split.
-    + rewrite IH1_i.
-      rewrite IH2_i.
-      reflexivity.
-    + rewrite fold_unfold_compile_v0_aux_Plus.
-      destruct (fetch_decode_execute_loop_v0_and_append_commute
-                  (compile_v0_aux ae1)
-                  (compile_v0_aux ae2 ++ ADD :: nil)
-                  nil) as [H _].
-      rewrite (H (n1 :: nil) IH1_c).
-      destruct (fetch_decode_execute_loop_v0_and_append_commute
-                  (compile_v0_aux ae2)
-                  (ADD :: nil)
-                  (n1 :: nil)) as [_ H1].
-      apply (H1 s2).
-  (* Plus msg nat *)
-  - right.
-    exists s1.
-    rewrite fold_unfold_evaluate_v0_Plus.
-    split.
-    + rewrite IH1_i.
-      reflexivity.
-    + rewrite fold_unfold_compile_v0_aux_Plus.
-      destruct (fetch_decode_execute_loop_v0_and_append_commute
-                  (compile_v0_aux ae1)
-                  (compile_v0_aux ae2 ++ ADD :: nil)
-                  nil) as [_ H].
-      apply (H s1).
-      exact IH1_c.
-  (* Plus msg msg *)
-  - right.
-    exists s1.
-    rewrite fold_unfold_evaluate_v0_Plus.
-    split.
-    + rewrite IH1_i.
-      reflexivity.
-    + rewrite fold_unfold_compile_v0_aux_Plus.
-      destruct (fetch_decode_execute_loop_v0_and_append_commute
-                  (compile_v0_aux ae1)
-                  (compile_v0_aux ae2 ++ ADD :: nil)
-                  nil) as [_ H].
-      apply (H s1).
-      exact IH1_c.
-  (* Minus nat nat *)
-  - admit.
-  (* Minus nat msg *)
-  - admit.
-  (* Minus msg nat *)
-  - admit.
-  (* Minus msg msg *)
-  - admit.
-Admitted.
+      rewrite -> H_n.
+      exact (fold_unfold_fetch_decode_execute_loop_v0_nil (n' :: ds)).
+    + intros s H_evaluate.
+      rewrite -> (fold_unfold_evaluate_v0_Literal n) in H_evaluate.
+      discriminate H_evaluate.
+  - split.
+    + intros n H_evaluate ds.
+      rewrite -> (fold_unfold_evaluate_v0_Plus ae1 ae2) in H_evaluate.
+      case (evaluate_v0 ae1) as [n1 | s1].
+      * case (evaluate_v0 ae2) as [n2 | s2].
+        -- rewrite -> (fold_unfold_compile_v0_aux_Plus ae1 ae2).
+           destruct (fetch_decode_execute_loop_v0_and_append_commute
+                       (compile_v0_aux ae1)
+                       (compile_v0_aux ae2 ++ ADD :: nil)
+                       ds) as [H _].
+           Check (IH1_OK n1 eq_refl ds).
+           rewrite -> (H (n1 :: ds) (IH1_OK n1 eq_refl ds)).
+           destruct (fetch_decode_execute_loop_v0_and_append_commute
+                       (compile_v0_aux ae2)
+                       (ADD :: nil)
+                       (n1 :: ds)) as [H1 _].
+           rewrite -> (H1 (n2 :: n1 :: ds) (IH2_OK n2 eq_refl (n1 :: ds))).
+           rewrite -> (fold_unfold_fetch_decode_execute_loop_v0_cons ADD nil (n2 :: n1 :: ds)).
+           unfold decode_execute_v0.
+           rewrite -> (fold_unfold_fetch_decode_execute_loop_v0_nil (n1 + n2 :: ds)).
+           injection H_evaluate as H_n.
+           rewrite H_n.
+           reflexivity.
+        -- discriminate H_evaluate.
+      * discriminate H_evaluate.
+    + intros s H_evaluate ds.
+      rewrite -> (fold_unfold_evaluate_v0_Plus ae1 ae2) in H_evaluate.
+      case (evaluate_v0 ae1) as [n1 | s1].
+      * case (evaluate_v0 ae2) as [n2 | s2].
+        -- discriminate H_evaluate.
+        -- rewrite -> (fold_unfold_compile_v0_aux_Plus ae1 ae2).
+           destruct (fetch_decode_execute_loop_v0_and_append_commute
+                       (compile_v0_aux ae1)
+                       (compile_v0_aux ae2 ++ ADD :: nil)
+                       ds) as [H _].
+           rewrite -> (H (n1 :: ds) (IH1_OK n1 eq_refl ds)).
+           destruct (fetch_decode_execute_loop_v0_and_append_commute
+                       (compile_v0_aux ae2)
+                       (ADD :: nil)
+                       (n1 :: ds)) as [_ H1].
+           apply (H1 s).
+           exact (IH2_KO s H_evaluate (n1 :: ds)).
+      * rewrite -> (fold_unfold_compile_v0_aux_Plus ae1 ae2).
+        destruct (fetch_decode_execute_loop_v0_and_append_commute
+                    (compile_v0_aux ae1)
+                    (compile_v0_aux ae2 ++ ADD :: nil)
+                    ds) as [_ H].
+        apply (H s).
+        exact (IH1_KO s H_evaluate ds).
+  - split.
+    + intros n H_evaluate ds.
+      rewrite -> (fold_unfold_evaluate_v0_Minus ae1 ae2) in H_evaluate.
+      case (evaluate_v0 ae1) as [n1 | s1].
+      * case (evaluate_v0 ae2) as [n2 | s2].
+        -- rewrite -> (fold_unfold_compile_v0_aux_Minus ae1 ae2).
+           destruct (fetch_decode_execute_loop_v0_and_append_commute
+                       (compile_v0_aux ae1)
+                       (compile_v0_aux ae2 ++ SUB :: nil)
+                       ds) as [H _].
+           Check (IH1_OK n1 eq_refl ds).
+           rewrite -> (H (n1 :: ds) (IH1_OK n1 eq_refl ds)).
+           destruct (fetch_decode_execute_loop_v0_and_append_commute
+                       (compile_v0_aux ae2)
+                       (SUB :: nil)
+                       (n1 :: ds)) as [H1 _].
+           rewrite -> (H1 (n2 :: n1 :: ds) (IH2_OK n2 eq_refl (n1 :: ds))).
+           rewrite -> (fold_unfold_fetch_decode_execute_loop_v0_cons SUB nil (n2 :: n1 :: ds)).
+           unfold decode_execute_v0.
+           case (n1 <? n2) eqn:H_lt.
+           ++ discriminate H_evaluate.
+           ++ rewrite -> (fold_unfold_fetch_decode_execute_loop_v0_nil (n1 - n2 :: ds)).
+              injection H_evaluate as H_n.
+              rewrite H_n.
+              reflexivity.
+        -- discriminate H_evaluate.
+      * discriminate H_evaluate.
+    + intros s H_evaluate ds.
+      rewrite -> (fold_unfold_evaluate_v0_Minus ae1 ae2) in H_evaluate.
+      case (evaluate_v0 ae1) as [n1 | s1].
+      * case (evaluate_v0 ae2) as [n2 | s2].
+        -- case (n1 <? n2) eqn:H_lt.
+           ++ rewrite -> (fold_unfold_compile_v0_aux_Minus ae1 ae2).
+              destruct (fetch_decode_execute_loop_v0_and_append_commute
+                          (compile_v0_aux ae1)
+                          (compile_v0_aux ae2 ++ SUB :: nil)
+                          ds) as [H _].
+              rewrite -> (H (n1 :: ds) (IH1_OK n1 eq_refl ds)).
+              destruct (fetch_decode_execute_loop_v0_and_append_commute
+                          (compile_v0_aux ae2)
+                          (SUB :: nil)
+                          (n1 :: ds)) as [H1 _].
+              destruct (fetch_decode_execute_loop_v0_and_append_commute
+                          (compile_v0_aux ae2)
+                          (SUB :: nil)
+                          (n1 :: ds)) as [H2 _].
+              rewrite -> (H1 (n2 :: n1 :: ds) (IH2_OK n2 eq_refl (n1 :: ds))).
+              rewrite -> (fold_unfold_fetch_decode_execute_loop_v0_cons SUB nil (n2 :: n1 :: ds)).
+              unfold decode_execute_v0.
+              rewrite H_lt.
+              injection H_evaluate as H_n.
+              rewrite <- H_n.
+              reflexivity.
+           ++ discriminate H_evaluate.
+        -- rewrite -> (fold_unfold_compile_v0_aux_Minus ae1 ae2).
+           destruct (fetch_decode_execute_loop_v0_and_append_commute
+                       (compile_v0_aux ae1)
+                       (compile_v0_aux ae2 ++ SUB :: nil)
+                       ds) as [H _].
+           rewrite -> (H (n1 :: ds) (IH1_OK n1 eq_refl ds)).
+           destruct (fetch_decode_execute_loop_v0_and_append_commute
+                       (compile_v0_aux ae2)
+                       (SUB :: nil)
+                       (n1 :: ds)) as [_ H1].
+           apply (H1 s).
+           exact (IH2_KO s H_evaluate (n1 :: ds)).
+      * rewrite -> (fold_unfold_compile_v0_aux_Minus ae1 ae2).
+        destruct (fetch_decode_execute_loop_v0_and_append_commute
+                    (compile_v0_aux ae1)
+                    (compile_v0_aux ae2 ++ SUB :: nil)
+                    ds) as [_ H].
+        apply (H s).
+        exact (IH1_KO s H_evaluate ds).
+Qed.
 
 Theorem the_commutative_diagram :
   forall (sp : source_program),
@@ -1191,33 +1224,13 @@ Theorem the_commutative_diagram :
 Proof.
   intros [ae].
   unfold interpret_v0, run_v0, compile_v0.
-  destruct (about_the_commutative_diagram ae) as [[n [H_nat_i H_nat_c]] | [s [H_msg_i H_msg_c]]].
-  - rewrite H_nat_i.
-    rewrite H_nat_c.
+  destruct (about_the_commutative_diagram ae) as [H_OK H_KO].
+  case (evaluate_v0 ae) as [n | s].
+  - rewrite -> (H_OK n eq_refl nil).
     reflexivity.
-  - rewrite H_msg_i.
-    rewrite H_msg_c.
+  - rewrite -> (H_KO s eq_refl nil).
     reflexivity.
 Qed.
-
-(* Theorem the_commutative_diagram : *)
-(*   forall (sp : source_program), *)
-(*     interpret_v0 sp = run_v0 (compile_v0 sp). *)
-(* Proof. *)
-(*   unfold interpret_v0, run_v0, compile_v0. *)
-(*   intros [ae]. *)
-(*   induction ae as [n | ae1 IH1 ae2 IH2 | ae1 IH1 ae2 IH2]. *)
-(*   - rewrite fold_unfold_evaluate_v0_Literal. *)
-(*     rewrite fold_unfold_compile_v0_aux_Literal. *)
-(*     rewrite fold_unfold_fetch_decode_execute_loop_v0_cons. *)
-(*     unfold decode_execute_v0. *)
-(*     rewrite fold_unfold_fetch_decode_execute_loop_v0_nil. *)
-(*     reflexivity. *)
-(*   - rewrite fold_unfold_evaluate_v0_Plus. *)
-(*     rewrite IH1. *)
-(*     rewrite IH2. *)
-(*     rewrite fold_unfold_compile_v0_aux_Plus. *)
-(*     rewrite fetch_decode_execute_loop_v0_and_append_commute. *)
 
 (* ********** *)
 
